Translation/Term.lean
@@ -2,6 +2,7 @@ import Core.Ty
 import Core.Term
 import Surface.Ty
 import Surface.Term
+import Core.Typing
 
 import Translation.Ty
 open LeanSubst
@@ -18,58 +19,61 @@ inductive Core.Translation.SynthTerm (G' : Core.GlobalEnv) (Δ' : Core.KindEnv) 
   Core.Ty -> Core.Term -> Prop where
 
 
-inductive Surface.Translation.Term (G : Surface.GlobalEnv) (G' : Core.GlobalEnv) :
+
+inductive Mode : Type where | chk | inf
+
+inductive Surface.Translation.Term (G : Surface.GlobalEnv) (G' : Core.GlobalEnv) : Mode ->
   Surface.KindEnv -> Surface.TyEnv -> Surface.Term -> Surface.Ty ->
   Core.KindEnv -> Core.TyEnv -> Core.Term -> Core.Ty -> Prop where
 | var  {Γ : Surface.TyEnv} :
-  Γ[x]? = some (A `=:> T) ->
-  Γ'[x]? = some (.arrow A' T') ->
+  Γ[x]? = some T ->
+  Γ'[x]? = some T' ->
   Translation.Ty G G' Δ T `★ Δ' T' ★ ->
-  Translation.Ty G G' Δ A `◯ Δ' A' ◯ ->
-  Core.Translation.SynthTerm G' Δ' Γ' A' d ->
-  Translation.Term G G' Δ Γ `#x T Δ' Γ' (#x ∘[ d ])  T'
+  Translation.Term G G' inf Δ Γ `#x T Δ' Γ' #x  T'
 | global :
   Surface.lookup_type G x = some T ->
   Core.lookup_type G' x = some T' ->
   Translation.Ty G G' Δ T `★ Δ' T' ★ ->
-  Translation.Term G G' Δ Γ g`#x T Δ' Γ' g#x T'
+  Translation.Term G G' inf Δ Γ g`#x T Δ' Γ' g#x T'
 | app :
   Translation.Ty G G' Δ A `★ Δ' A' ★ ->
-  Translation.Term G G' Δ Γ f (A `-:> B) Δ' Γ' f' (A' -:> B') ->
-  Translation.Term G G' Δ Γ a A Δ' Γ' a' A' ->
-  Translation.Term G G' Δ Γ f (A `-:> B) Δ' Γ' f' B'
+  Translation.Term G G' inf Δ Γ f (A `-:> B) Δ' Γ' f' (A' -:> B') ->
+  Translation.Term G G' chk Δ Γ a A Δ' Γ' a' A' ->
+  Translation.Term G G' inf Δ Γ (f `• a) B Δ' Γ' (f' • a') B'
 | appP :
   Translation.Ty G G' Δ A `◯ Δ' A' ◯ ->
-  Translation.Term G G' Δ Γ f (A `=:> B) Δ' Γ' f' (A' -:> B') ->
-  Core.Translation.SynthTerm G' Δ' Γ' A' a' ->
-  Translation.Term G G' Δ Γ f B Δ' Γ' (f' ∘[ a' ]) B'
+  Translation.Term G G' inf Δ Γ f (A `=:> B) Δ' Γ' f' (A' -:> B') ->
+  Translation.Term G G' chk Δ Γ a A Δ' Γ' a' A' ->
+  Translation.Term G G' inf Δ Γ (f `• a) B Δ' Γ' (f' ∘[ a' ]) B'
 | lam :
   Translation.Ty G G' Δ A `★ Δ' A' ★ ->
-  Translation.Term G G' Δ (A::Γ) t B Δ' (A'::Γ') t' B' ->
-  Translation.Term G G' Δ Γ (λˢ[A] t) (A `-:> B) Δ' Γ' (λ[A'] t') (A' -:> B')
+  Translation.Term G G' chk Δ (A::Γ) t B Δ' (A'::Γ') t' B' ->
+  Translation.Term G G' chk Δ Γ (λˢ[A] t) (A `-:> B) Δ' Γ' (λ[A'] t') (A' -:> B')
+| lamt :
+  Translation.Ty G G' (K::Δ) P `★ (K.translate::Δ') P' ★ ->
+  Translation.Term G G' ch (K::Δ) (Γ.map (·[+1])) t P (K.translate :: Δ') (Γ'.map (·[+1])) t' P' ->
+  Translation.Term G G' chk Δ Γ (Λˢ[K] t) (`∀[K] P) Δ' Γ' (Λ[K.translate] t') (∀[K.translate] P')
+
 | mtch (CTy : Vect n Surface.Ty) (CTy' : Vect n Core.Ty)
        (PTy : Vect n Surface.Ty) (PTy' : Vect n Core.Ty)
        (pats : Vect n Surface.Term) (pats' : Vect n Core.Term)
        (cs : Vect n Surface.Term) (cs' : Vect n Core.Term) :
-  Translation.Term G G' Δ Γ s R Δ' Γ' s' R' ->
+  Translation.Term G G' inf Δ Γ s R Δ' Γ' s' R' ->
   ValidTyHeadVariable R (is_data G) ->
-  Translation.Term G G' Δ Γ c T Δ' Γ' c' T' -> -- catch all term is of type T
+  Translation.Term G G' inf  Δ Γ c T Δ' Γ' c' T' -> -- catch all term is of type T
   (∀ i, ValidHeadVariable (pats i) (is_ctor G)) -> -- patterns are of the right shape
-  (∀ i, Translation.Term G G' Δ Γ (pats i) (PTy i) Δ' Γ' (pats' i) (PTy' i)) -> -- each pattern has a type
+  (∀ i, Translation.Term G G' chk Δ Γ (pats i) (PTy i) Δ' Γ' (pats' i) (PTy' i)) -> -- each pattern has a type
   (∀ i, StableTypeMatch Δ (PTy i) R) -> -- the pattern type has a return type that matches datatype
-  (∀ i, Translation.Term G G' Δ Γ (cs i) (PTy i) Δ' Γ' (cs' i) (CTy' i)) -> -- each case match has a type
+  (∀ i, Translation.Term G G' chk Δ Γ (cs i) (PTy i) Δ' Γ' (cs' i) (CTy' i)) -> -- each case match has a type
   (∀ i, PrefixTypeMatch Δ (PTy i) (CTy i) T) -> -- patten type and case type
-  Translation.Term G G' Δ Γ (matchˢ! s pats cs c) T Δ' Γ' (match! n s' pats' cs' c') T'
-| lamt :
-  Translation.Ty G G' (K::Δ) P `★ (K.translate::Δ') P' ★ ->
-  Translation.Term G G' (K::Δ) (Γ.map (·[+1])) t P (K.translate :: Δ') (Γ'.map (·[+1])) t' P' ->
-  Translation.Term G G' Δ Γ (Λˢ[K] t) (`∀[K] P) Δ' Γ' (Λ[K.translate] t') (∀[K.translate] P')
+  Translation.Term G G' chk Δ Γ (matchˢ! n R s pats cs c) T Δ' Γ' (match! n s' pats' cs' c') T'
+
 | annot :
   Translation.Ty G G' Δ Ta `★ Δ' Ta' ★ ->
   Translation.Ty G G' Δ Tb `★ Δ' Tb' ★ ->
   Core.Translation.SynthTerm G' Δ' Γ' (Ta' ~[★]~ Tb') c ->
-  Translation.Term G G' Δ Γ t Ta Δ' Γ' t' Ta' ->
-  Translation.Term G G' Δ Γ (.annot t Ta) Tb Δ' Γ' (t' ▹ c) Tb'
+  Translation.Term G G' chk Δ Γ t Ta Δ' Γ' t' Ta' ->
+  Translation.Term G G' inf Δ Γ (.annot t Ta) Tb Δ' Γ' (t' ▹ c) Tb'
 
 
 @[simp, grind]
@@ -91,7 +95,7 @@ def Surface.Term.translate (G : Core.GlobalEnv) (Δ : Core.KindEnv) (Γ : Core.T
   let t1' <- t1.translate G Δ Γ
   let t2' <- t2.translate
   return (t1' •[ t2' ])
-| .match (n := n) s ps cs d => do
+| .match (n := n) _ s ps cs d => do
   let s' <- s.translate G Δ Γ
   let ops' : Vect n (Option Core.Term) := (λ i => (ps i).translate G Δ Γ)
   let ps' <- ops'.seq
@@ -101,30 +105,26 @@ def Surface.Term.translate (G : Core.GlobalEnv) (Δ : Core.KindEnv) (Γ : Core.T
   return match! n s' ps' cs' d'
 | .annot t _ => do
   t.translate G Δ Γ
-| .hole T => T.translate.synth_term G Δ Γ
+
 
 
 -- @[simp, grind]
-def Surface.Term.type_directed_translate (G : Core.GlobalEnv) (Δ : Core.KindEnv) (Γ : Core.TyEnv) (τ : Surface.Ty):
+def Surface.Term.type_directed_translate
+  (G : Core.GlobalEnv) (Δ : Core.KindEnv) (Γ : Core.TyEnv) (τ : Surface.Ty) :
   Surface.Term -> Option Core.Term
-| `#x => do
-  match τ with
-  | .then A B =>
-    let d <- Core.Ty.synth_term G Δ Γ A.translate
-    return (#x ∘[d])
+| `#x =>
+  match Γ[x]? with
+  | some τ' => do
+    let c <- (τ' ~[★]~ τ.translate).synth_term G Δ Γ
+    return (#x ▹ c)
   | _ => none
 
-| g`#x => do
-  match τ with
-  | .then A B =>
-    let d <- Core.Ty.synth_term G Δ Γ A.translate
-    return (g#x ∘[d])
-  | _ => none
-
-  -- match Γ[x]? with
-  -- | some τ' =>
-  --   if τ.translate == τ' then return #x else none
-  -- | _ =>  none
+| g`#x =>
+  match Core.lookup_type G x with
+  | some τ' => do
+    let c <- (τ' ~[★]~ τ.translate).synth_term G Δ Γ
+    return (g#x ▹ c)
+  | _ =>  none
 | .lamt K t => do
   match τ with
   | .all K' τ' =>
@@ -138,8 +138,8 @@ def Surface.Term.type_directed_translate (G : Core.GlobalEnv) (Δ : Core.KindEnv
     if A == A' then return λ[A.translate] t' else none
   | _ => none
 -- Elimination forms are a little annoying
-| .match (n := n) (annot s sτ) ps cs d => do -- also maybe store the type of the scrutinee to eliminate
-  let s' <- s.type_directed_translate G Δ Γ sτ
+| .match (n := n) R s ps cs d => do
+  let s' <- s.type_directed_translate G Δ Γ R
   let ops' : Vect n (Option Core.Term) := (λ i => (ps i).translate G Δ Γ)
   let ps' <- ops'.seq
   let ocs' : Vect n (Option Core.Term) := (λ i => (cs i).translate G Δ Γ)
@@ -180,3 +180,55 @@ def Surface.Term.type_directed_translate (G : Core.GlobalEnv) (Δ : Core.KindEnv
 -- · omega
 -- · have lem := Spine.elem_size_le_term sp_prf (.term t) prf; simp [SpineElem.size] at lem; exact lem
 -- )
+
+def Surface.Term.type_inf_translate
+  (G : Surface.GlobalEnv) (Δ : Surface.KindEnv) (Γ : Surface.TyEnv)
+  (G' : Core.GlobalEnv) (Δ' : Core.KindEnv) (Γ' : Core.TyEnv) :
+  Surface.Term -> Option (Core.Term × Surface.Ty × Core.Ty) := by
+
+sorry
+
+
+def Surface.Term.type_chk_translate -- Ideally should take τ as input, normal translate may return τ (inf mode)
+  (G : Surface.GlobalEnv) (Δ : Surface.KindEnv) (Γ : Surface.TyEnv) (τ : Surface.Ty)
+  (G' : Core.GlobalEnv) (Δ' : Core.KindEnv) (Γ' : Core.TyEnv) (τc : Core.Ty) :
+  Surface.Term -> Option Core.Term
+| `#x =>
+  match Γ'[x]? with
+  | some τ' => do
+    let c <- (τ' ~[★]~ τ.translate).synth_term G' Δ' Γ'
+    return (#x ▹ c)
+  | _ => none
+
+| g`#x =>
+  match Core.lookup_type G' x with
+  | some τ' => do
+    let c <- (τ' ~[★]~ τ.translate).synth_term G' Δ' Γ'
+    return (g#x ▹ c)
+  | _ =>  none
+| .lamt K t => do
+  match τ, τc with
+  | .all K' τ', .all Kc τc' =>
+    let t' <- t.type_chk_translate G (K::Δ) (Γ.map (·[+1])) τ' G' (Kc :: Δ') (Γ'.map (·[+1])) τc'
+    if K.translate == Kc && K' == K then return (Λ[Kc] t') else none
+  | _, _ => none
+| .lam A' t => do
+  match τ, τc with
+  | .arrow A B, .arrow Ac Bc =>
+    let t' <- t.type_chk_translate G Δ (A::Γ) B G' Δ' (Ac :: Γ') Bc
+    if A == A'  && A.translate == Ac then return λ[A.translate] t' else none
+  | _,_ => none
+-- Elimination forms are a little annoying
+| .match (n := n) R s ps cs d => do
+  let s' <- s.type_chk_translate G Δ Γ R G' Δ' Γ' R.translate
+  let ops' : Vect n (Option Core.Term) := (λ i => (ps i).translate G' Δ' Γ')
+  let ps' <- ops'.seq
+  let ocs' : Vect n (Option Core.Term) := (λ i => (cs i).translate G' Δ' Γ')
+  let cs' <- ocs'.seq
+  let d' <- d.type_chk_translate G Δ Γ τ G' Δ' Γ' τ.translate
+  return match! n s' ps' cs' d'
+| .annot t τt => do
+  let t' <- t.type_chk_translate G Δ Γ τt G' Δ' Γ' τt.translate
+  let c <- Core.Ty.synth_coercion G' Δ' Γ' τt.translate τ.translate
+  return t' ▹ c
+| _ => none
