Surface/Term/Substitution.lean
@@ -36,9 +36,8 @@ def Term.rmap (r : Ren) : Term -> Term
 | lam A t => lam A (rmap r.lift t)
 | app t1 t2 => app (rmap r t1) (rmap r t2)
 | appt t1 t2 => appt (rmap r t1) t2
-| .match t1 t2 t3 t4 => .match (rmap r t1) (rmap r <$> t2) (rmap r <$> t3) (rmap r t4)
+| .match n t0 t1 t2 t3 t4 => .match n t0 (rmap r t1) (rmap r <$> t2) (rmap r <$> t3) (rmap r t4)
 | annot t1 A => annot (rmap r t1) A
-| hole τ => hole τ
 
 instance instRenMap_Term : RenMap Term where
   rmap := Term.rmap
@@ -51,9 +50,8 @@ def Term.Ty.smap (σ : Subst Ty) : Term -> Term
 | appt t1 t2 => appt (smap σ t1) t2[σ:_]
 | lamt A t => lamt A (smap σ.lift t)
 | lam A t => lam A[σ:_] (smap σ t)
-| .match t1 t2 t3 t4  => .match (smap σ t1) (λ i => smap σ (t2 i)) (λ i => smap σ (t3 i)) (smap σ t4)
+| .match n t0 t1 t2 t3 t4  => .match n t0 (smap σ t1) (λ i => smap σ (t2 i)) (λ i => smap σ (t3 i)) (smap σ t4)
 | annot t1 A => annot (smap σ t1) A[σ:_]
-| hole τ => hole τ[σ:_]
 
 instance instSubstMap_TermTy : SubstMap Term Ty where
   smap := Term.Ty.smap
@@ -66,9 +64,8 @@ def Term.smap (σ : Subst Term) : Term -> Term
 | appt t1 t2 => appt (smap σ t1) t2
 | lamt A t => lamt A (smap (σ ◾ +1@Ty) t)
 | lam A t => lam A (smap σ.lift t)
-| .match t1 t2 t3 t4 => .match (smap σ t1) (λ i => smap σ (t2 i)) (λ i => smap σ (t3 i)) (smap σ t4)
+| .match n t0 t1 t2 t3 t4 => .match n t0 (smap σ t1) (λ i => smap σ (t2 i)) (λ i => smap σ (t3 i)) (smap σ t4)
 | annot t1 A => annot (smap σ t1) A
-| hole τ => hole τ
 
 
 
@@ -95,10 +92,6 @@ theorem Term.subst_appt : (appt t1 t2)[σ:Term] = appt t1[σ:_] t2 := by
 theorem Term.subst_annoτ : (annot t1 t2)[σ:Term] = annot t1[σ:_] t2 := by
   simp [SubstMap.smap]
 
-@[simp]
-theorem Term.subst_hole : (hole t1)[σ:Term] = hole t1 := by
-  simp [SubstMap.smap]
-
 
 @[simp]
 theorem Term.subst_lamt : (lamt A t)[σ:Term] = lamt A t[σ ◾ +1@Ty:_] := by
@@ -110,7 +103,7 @@ theorem Term.subst_lam : (lam A t)[σ:Term] = lam A t[σ.lift:_] := by
 
 @[simp]
 theorem Term.subst_match
-  : (matchˢ! t1 t2 t3 t4)[σ:Term] = matchˢ! t1[σ:_] (λ i => (t2 i)[σ:_]) (λ i => (t3 i)[σ:_]) (t4[σ:_])
+  : (matchˢ! n t0 t1 t2 t3 t4)[σ:Term] = matchˢ! n t0 t1[σ:_] (λ i => (t2 i)[σ:_]) (λ i => (t3 i)[σ:_]) (t4[σ:_])
 := by
   simp [SubstMap.smap]
 
@@ -149,14 +142,10 @@ theorem Term.Ty.subst_lam : (lam A t)[σ:Ty] = lam A[σ:_] t[σ:_] := by
 theorem Term.Ty.subst_annoτ : (annot t A)[σ:Ty] = annot t[σ:_] A[σ:_] := by
   simp [SubstMap.smap]
 
-@[simp]
-theorem Term.Ty.subst_hole : (hole τ)[σ:Ty] = hole τ[σ:_] := by
-  simp [SubstMap.smap]
-
 
 @[simp]
 theorem Term.Ty.subst_match
-  : (matchˢ! t1 ps t2 t3)[σ:Ty] = matchˢ! t1[σ:_] (λ i => (ps i)[σ:_]) (λ i => (t2 i)[σ:_]) t3[σ:_]
+  : (matchˢ! n t0 t1 ps t2 t3)[σ:Ty] = matchˢ! n t0 t1[σ:_] (λ i => (ps i)[σ:_]) (λ i => (t2 i)[σ:_]) t3[σ:_]
 := by
   simp [SubstMap.smap]
 
